SystemFD/Metatheory/Cannonicity.lean
@@ -1,0 +1,136 @@
+import SystemFD.Term
+import SystemFD.Ctx
+import SystemFD.Judgment
+import SystemFD.Metatheory.Classification
+import SystemFD.Metatheory.FrameWf
+import SystemFD.Metatheory.Inversion
+import SystemFD.Reduction
+
+inductive Val : Ctx Term -> Term -> Prop where
+| app : t.neutral_form = .some (n, ts)
+      -> (Γ.is_stable_red n)
+      -> Val Γ t
+| lam :  Val Γ (`λ[a] b)
+| lamt : Val Γ (Λ[A] b)
+| refl : Val Γ (refl! _)
+| star : Val Γ ★
+| arr :  Val Γ (A -t> B)
+| arrk : Val Γ (A -k> B)
+| all : Val Γ (∀[A]B)
+| eq : Val Γ (A ~ B)
+
+theorem refl_var_spine_lemma :
+  Γ.is_stable_red n ->
+  Γ ⊢ (#n).apply_spine sp : (A ~ B) ->
+  False
+:= by
+intro j1 j2
+have lem := inversion_apply_spine j2
+cases lem; case _ C lem =>
+cases lem; case _ h1 h2 =>
+cases h2; case _ j3 j4 =>
+  have lem := classification_lemma j2 <;> simp at lem
+  cases lem
+  case _ lem => cases lem
+  case _ lem =>
+    cases lem; case _ K lem =>
+    cases lem.2; case _ q1 q2 q3 =>
+      apply ctx_get_var_no_spine_eq_type j3 j1
+      rw [j4]; apply lem.2; apply h1
+
+theorem refl_is_val :
+  Γ ⊢ η : (A ~ B) ->
+  Val Γ η ->
+  η = refl! A ∧ A = B
+:= by
+intros ηJ vη; induction vη;
+any_goals(solve | cases ηJ)
+case _ Γ t n ts tnf n_stable =>
+     symm at tnf; replace tnf := Term.neutral_form_law tnf;
+     subst tnf;
+     exfalso;
+     apply (refl_var_spine_lemma n_stable ηJ);
+case _ => cases ηJ; case _ fJ =>
+  have lem := classification_lemma fJ; simp at lem; cases lem;
+  case _ h => cases h; case _ h => cases h
+  case _ h => apply And.intro rfl rfl
+
+theorem cannonical_ctor_head :
+  Γ ⊢ #h : T ->
+  Γ ⊢ T : ★ ->
+  ValidCtor Γ T ->
+  Γ.is_stable_red h ->
+  Γ.is_ctor h := by
+intros tJ tstar vctor n_stable;
+cases tJ; case _ wf h1 =>
+  have h2 := @frame_wf_by_index Γ h wf;
+  have h3 := @frame_wf_implies_typed_var Γ h T h2 h1;
+  generalize fh : Γ d@ h = f at *;
+  unfold Frame.get_type at h1;
+  split at h1;
+  any_goals (solve | simp at *)
+  all_goals (unfold Ctx.is_stable_red at n_stable; unfold Frame.is_stable_red at n_stable)
+  any_goals (solve |  rw [fh] at n_stable; simp at n_stable)
+  case _ =>
+    injection h1 with h1; cases h1;
+    have lem := ctx_get_var_type wf fh;
+    have uniq := uniqueness_of_types tstar lem;
+    cases uniq;
+  case _ =>
+    injection h1 with h1; cases h1;
+    have lem := ctx_get_datatype_kind wf fh;
+    have uniq := uniqueness_of_types tstar lem;
+    cases uniq;
+  case _ => unfold Ctx.is_ctor; unfold Frame.is_ctor; rw [fh]
+  case _ =>
+    injection h1 with h1; cases h1;
+    have lem := ctx_get_opent_kind wf fh;
+    have uniq := uniqueness_of_types tstar lem;
+    cases uniq;
+  case _ =>
+    injection h1 with h1; cases h1;
+    cases h2; case _ vit =>
+    exfalso
+    apply datatype_opent_distinct vctor vit
+
+
+
+theorem cannonical_insttype_head :
+  Γ ⊢ #h : T ->
+  Γ ⊢ T : ★ ->
+  ValidInstType Γ T ->
+  Γ.is_stable_red h ->
+  Γ.is_insttype h := by
+intros tJ tstar vctor n_stable;
+cases tJ; case _ wf h1 =>
+  have h2 := @frame_wf_by_index Γ h wf;
+  have h3 := @frame_wf_implies_typed_var Γ h T h2 h1;
+  generalize fh : Γ d@ h = f at *;
+  unfold Frame.get_type at h1;
+  split at h1;
+  any_goals (solve | simp at *)
+  all_goals (unfold Ctx.is_stable_red at n_stable; unfold Frame.is_stable_red at n_stable)
+  any_goals (solve |  rw [fh] at n_stable; simp at n_stable)
+  case _ =>
+    injection h1 with h1; cases h1;
+    have lem := ctx_get_var_type wf fh;
+    have uniq := uniqueness_of_types tstar lem;
+    cases uniq;
+  case _ =>
+    injection h1 with h1; cases h1;
+    have lem := ctx_get_datatype_kind wf fh;
+    have uniq := uniqueness_of_types tstar lem;
+    cases uniq;
+  case _ =>
+    injection h1 with h1; cases h1;
+    cases h2; case _ vit =>
+      exfalso
+      apply datatype_opent_distinct vit vctor
+  case _ =>
+    injection h1 with h1; cases h1;
+    have lem := ctx_get_opent_kind wf fh;
+    have uniq := uniqueness_of_types tstar lem;
+    cases uniq;
+  case _ =>
+    injection h1 with h1; cases h1;
+    simp; rw [fh]; unfold Frame.is_insttype; simp;
